Here, we talk about product rule with 3 functions.

We know the rule with 2 functions:
$$
(uv)' = u'v + u(v')
$$
Just use it:
$$
\begin{aligned}
(uvw)' &= [u(vw)]' 
\\&= (u')(vw) + u(vw)'
\\&=(u')vw + u(v')w +uv(w')
\end{aligned}
$$
It looks like we take derivative of the functions one by one and the others just stay still.

Example: Get the derivative of $f(x) = x^2\sin x \cos x$. It's easy to use the formula we find to solve this question.
$$
f'(x) = 2x \sin x \cos x + x^2 \cos^2 x - x^2 \sin^2 x
$$
Actually, we can rewrite this using trig identity but it's a sufficient answer.
